examples/FAI.v
@@ -10,6 +10,7 @@ Require Import LinCCAL.
 Require Import LTS.
 Require Import Lang.
 Require Import Semantics.
+Require Import Logics.
 Require Import Assertion.
 Require Import TPSimulation.
 Require Import RGILogic.
@@ -50,7 +51,7 @@ Module FAIImpl.
     inl rel >= _ =>
     Ret c.
 
-  Definition assertion := @Assertion _ _ (li_lts E) (li_lts F).
+  Definition assertion := @Assertion (@ProofState _ _ (li_lts E) (li_lts F)).
   Definition rg_relation := @RGRelation _ _ (li_lts E) (li_lts F).
 
   Open Scope rg_relation_scope.
